formal/IO.thy
@@ -1,0 +1,46 @@
+theory IO
+  imports Types
+begin
+
+abbreviation noouts :: "outputs" where
+"noouts  \<equiv> \<lambda>(ip,dt) . \<lambda>ot . None"
+
+definition blankouts :: "outvalues" where
+"blankouts \<equiv> \<lambda>x . None"
+declare blankouts_def [simp]
+
+definition blankdata :: "data" where
+"blankdata \<equiv> \<lambda>x . None"
+declare blankdata_def [simp]
+
+definition noupdates :: "updates" where
+"noupdates  \<equiv> \<lambda>(ip,dt) . dt"
+declare noupdates_def [simp]
+
+abbreviation trueguard :: "guard" where
+"trueguard \<equiv> \<lambda>x. True"
+
+definition blankips :: "inputs" where
+"blankips \<equiv> \<lambda>x . None"
+declare blankips_def [simp]
+
+(* Stuff for making traces from simpler to type stuff... *)
+definition overwrite :: "('a \<Rightarrow> 'b) \<Rightarrow> ('a * 'b) \<Rightarrow> ('a \<Rightarrow> 'b)" (infix "\<oplus>" 50) where
+"overwrite \<equiv> \<lambda>f . \<lambda>(k,v) . \<lambda>kk . if kk = k then v else f(kk)"
+declare overwrite_def[simp]
+
+primrec make_trace_step :: "inputs \<Rightarrow> valuetype list => int \<Rightarrow> inputs" where
+"make_trace_step ips [] _ = ips"
+|"make_trace_step ips (i#is) n = make_trace_step (ips \<oplus> (n,Some i)) is (n+1)"
+
+(* Make a trace (i.e. a list of input partial functions) from a list of literals *)
+primrec make_trace :: "valuetype list list \<Rightarrow> trace" where
+"make_trace [] = []"
+|"make_trace (t#ts) = (make_trace_step blankips t 0)#(make_trace ts)"
+
+(* Make an observation (i.e. a list of output partial functions) from a list of literals *)
+primrec make_obs :: "valuetype list list \<Rightarrow> observation" where
+"make_obs [] = []"
+|"make_obs (t#ts) = (make_trace_step blankouts t 1)#(make_obs ts)"
+
+end
