formal/Vend.thy
@@ -1,0 +1,73 @@
+theory Vend
+  imports EFSM
+begin
+
+definition t1 :: "transition" where
+"t1 \<equiv> (\<lambda>(ip,dt) . ip(0) = Some (Inr ''select''), noouts, \<lambda>(ip,dt) . dt \<oplus> (1,ip(1)))"
+
+abbreviation u1 :: "updates" where
+"u1 \<equiv> \<lambda>(ip,dt) . dt \<oplus> (2,(dt(2)) + (ip(1)))"
+
+definition t2 :: "transition" where
+"t2 \<equiv> (\<lambda>(ip,dt) . ip(0) = Some (Inr ''coin''), noouts, u1)"
+
+abbreviation g1 :: "guard" where
+"g1 \<equiv> \<lambda>(ip,dt) . (ip(0) = Some (Inr ''vend'')) \<and> (dt(2)) \<ge> (Some (Inl 100))"
+
+definition t3 :: "transition" where
+"t3 \<equiv> (g1, \<lambda>(ip,dt) . blankouts \<oplus> (1,dt(1)), noupdates)"
+
+definition vend :: "efsm" where
+"vend \<equiv> \<lparr> S = [1,2,3],
+          s0 = 1,
+          d0 = ((blankdata \<oplus> (1,Some (Inl 0))) \<oplus> (2,Some (Inl 0))),
+          M = \<lambda> (a,b) . 
+              if (a,b) = (1,2) then [t1]
+              else if (a,b) = (2,2) then [t2]
+              else if (a,b) = (2,3) then [t3]
+              else []
+         \<rparr>"
+
+lemma "possible_steps vend 1 blankips blankdata == []"
+  by (simp add: vend_def t1_def)
+lemma "possible_steps vend 1 (blankips \<oplus> (0,Some (Inr ''select''))) blankdata == [(2,t1)]"
+  by (simp add: vend_def t1_def)
+lemma "possible_steps vend 2 (blankips \<oplus> (0,Some (Inr ''coin''))) blankdata == [(2,t2)]"
+  by (simp add: vend_def t2_def t3_def)
+lemma "possible_steps vend 2 (blankips \<oplus> (0,Some (Inr ''vend''))) blankdata \<noteq> [(3,t3)]"
+  by (simp add: vend_def t2_def t3_def)
+lemma "possible_steps vend 2 (blankips \<oplus> (0,Some (Inr ''vend''))) (blankdata \<oplus> (1,Some (Inl 50))) \<noteq> [(3,t3)]"
+  by (simp add: vend_def t2_def t3_def)
+lemma "possible_steps vend 2 (blankips \<oplus> (0,Some (Inr ''vend''))) (blankdata \<oplus> (1,Some (Inl 99))) \<noteq> [(3,t3)]"
+  by (simp add: vend_def t2_def t3_def)
+lemma "possible_steps vend 2 (blankips \<oplus> (0,Some (Inr ''vend''))) ((blankdata \<oplus> (1,Some (Inl 42))) \<oplus> (2,Some (Inl 100))) = [(3,t3)]"
+  by (simp add: vend_def t2_def t3_def)
+
+lemma "step vend 2 ((blankips \<oplus> (0,Some (Inr ''coin''))) \<oplus> (1,Some (Inl 50))) (blankdata \<oplus> (2,Some (Inl 0))) = Some (2, blankouts, (blankdata \<oplus> (2,Some (Inl 50))))"
+  by (simp add: vend_def step_def t2_def t3_def) auto
+
+definition tr1 :: "trace" where
+"tr1 \<equiv> make_trace [[(Inr ''select''),(Inr ''coke'')],[(Inr ''coin''),(Inl 50)],[(Inr ''coin''),(Inl 50)],[(Inr ''vend'')]]"
+definition ob1 :: "observation" where
+"ob1 \<equiv> make_obs [[],[],[],[(Inr ''coke'')]]"
+
+definition tr2 :: "trace" where
+"tr2 \<equiv> make_trace [[(Inr ''select''),(Inr ''coke'')],[(Inr ''coin''),(Inl 50)],[(Inr ''coin''),(Inl 50)]]"
+definition ob2 :: "observation" where
+"ob2 \<equiv> make_obs [[],[],[]]"
+
+definition tr3 :: "trace" where
+"tr3 \<equiv> make_trace [[(Inr ''select''),(Inl 42)]]"
+definition ob3 :: "observation" where
+"ob3 \<equiv> make_obs [[]]"
+
+lemma "observe vend tr3 = ob3" 
+ by (simp add: vend_def tr3_def observe_def t1_def fst_def ob3_def)  
+
+lemma "observe vend tr2 = ob2" 
+  by (simp add: vend_def tr2_def observe_def ob2_def t1_def t2_def t3_def)  
+  
+lemma "observe vend tr1 = ob1"
+  by (simp add: vend_def tr1_def observe_def ob1_def t1_def t2_def t3_def)  
+
+end
