formal/Vend2.thy
@@ -1,0 +1,20 @@
+theory Vend2
+  imports Vend
+begin
+
+definition vend2 :: "efsm" where
+"vend2 \<equiv> \<lparr>S = [1,2,3,4],
+          s0 = 1,
+          d0 = ((blankdata \<oplus> (1,Some (Inl 0))) \<oplus> (2,Some (Inl 0))),
+          M = \<lambda>(s,s') . 
+                if (s,s') = (1,2) then [t1]
+                else if (s,s') = (2,3) then [t2]
+                else if (s,s') = (3,3) then [t2]
+                else if (s,s') = (3,4) then [t3]
+                else []
+          \<rparr>"
+
+theorem "equiv vend2 vend tr1"
+  by (simp add: t1_def t2_def t3_def vend_def vend2_def equiv_def observe_def tr1_def)
+  
+end
